clightplus_examples/vector/vector01proof_vector_destruct.v
@@ -1,0 +1,187 @@
+Require Import CoqlibCCR.
+Require Import Any.
+Require Import STS.
+Require Import Behavior.
+Require Import ModSem.
+Require Import SimModSem.
+Require Import PCM.
+Require Import HoareDef.
+Require Import STB.
+Require Import HTactics ProofMode.
+Require Import HSim IProofMode.
+Require Import ClightPlusSkel ClightPlusExprgen ClightPlusgen.
+Require Import ClightPlusMem0 ClightPlusMem1 ClightPlusMemAux.
+Require Import CProofMode CIProofMode.
+Require Import vector.
+Require Import vector0.
+Require Import vector1.
+Require Import PtrofsArith.
+From Coq Require Import Program.
+From compcert Require Import Clightdefs.
+Require Import vector_auxiliary.
+
+Section PROOF.
+
+  Import ClightPlusMem1.
+
+  Context `{@GRA.inG pointstoRA Σ}.
+  Context `{@GRA.inG allocatedRA Σ}.
+  Context `{@GRA.inG blocksizeRA Σ}.
+  Context `{@GRA.inG blockaddressRA Σ}.
+
+  Variable GlobalStb : Sk.t -> gname -> option fspec.
+  Hypothesis STBINCL : forall sk, stb_incl (to_stb vectorStb) (GlobalStb sk).
+  Hypothesis MEMINCL : forall sk, stb_incl (to_stb MemStb) (GlobalStb sk).
+
+  Variable sk: Sk.t.
+  Hypothesis SKINCL1 : Sk.le (vector_compiled.(Mod.sk)) sk.
+  Hypothesis SKINCL2 : Sk.le mfsk sk.
+  Hypothesis SKWF : Sk.wf sk.
+
+  Let ce := Maps.PTree.elements (prog_comp_env prog).
+
+  Lemma sim_vector_destruct :
+    sim_fnsem wf top2
+      ("vector_destruct", fun_to_tgt "vector" (GlobalStb sk) (mk_pure vector_destruct_spec))
+      ("vector_destruct", cfunU (decomp_func sk ce f_vector_destruct)).
+  Proof.
+    Local Opaque encode_val.
+    Local Opaque cast_to_ptr.
+    econs; ss. red.
+
+    unfold prog, mkprogram in ce.
+    destruct (build_composite_env' composites I). ss.
+    get_composite ce e. fold vector._vector in get_co.
+
+    pose proof (incl_incl_env SKINCL1) as SKINCLENV1. unfold incl_env in SKINCLENV1.
+    pose proof (incl_incl_env SKINCL2) as SKINCLENV2. unfold incl_env in SKINCLENV2.
+    pose proof sk_incl_gd as SKINCLGD.
+
+    apply isim_fun_to_tgt; auto. i. simpl in x.
+    destruct x as [[[[[[[v esize] capacity] length] cells] mᵥ] tgᵥ] qᵥ].
+    unfold decomp_func, function_entry_c; ss.
+    set (HIDDEN := hide 1).
+
+    iIntros "[INV PRE]".
+    iDestruct "PRE" as "[[% V] %]".
+    clarify. hred_r.
+
+    unhide. hred_r. remove_tau.
+    unhide. hred_r. remove_tau.
+    hexploit SKINCLENV2.
+    { right. left. ss. }
+    i. des. rewrite FIND. hred_r.
+
+    iPoseProof (is_vector_is_ptr_val with "V") as "%".
+    rewrite H3. hred_r. rewrite H3. hred_r.
+    replace (alist_find vector._vector ce) with (Some co).
+    hred_r.
+    replace (ClightPlusExprgen.field_offset ce _data (co_members co))
+      with (Errors.OK 0%Z)
+      by (rewrite co_co_members; ss).
+    change Archi.ptr64 with true. ss. hred_r.
+
+    unfold is_vector.
+    iDestruct "V" as (data m_data unused_length unused) "[% [V [LPT [DATA_HO DATA_PT]]]]". des.
+
+    iApply isim_apc. iExists (Some (3: Ord.t)).
+    iPoseProof (accessor_is_vector_handler_data with "V") as (ofsᵥ) "[DATA V_RECOVER]".
+    iApply isim_ccallU_load.
+    { ss. }
+    { eapply OrdArith.lt_from_nat. lia. }
+    { instantiate (1:=2%ord). eapply OrdArith.lt_from_nat. lia. }
+    iSplitL "INV DATA". { iSplitL "INV"; done. }
+    iIntros (st_src0 st_tgt0) "[INV DATA]".
+    iPoseProof (offset_is_ptr with "DATA_HO") as "%".
+    iPoseProof ("V_RECOVER" with "[DATA]") as "V".
+    { iFrame; ss. }
+    clear ofsᵥ.
+
+    iPoseProof (offset_is_ptr with "DATA_HO") as "%".
+    hred_r.
+    rewrite (decode_encode_ptr _ H13).
+    rewrite (cast_to_ptr_ptr _ H13).
+    hred_r.
+
+    des_if; ss. hred_r.
+    rewrite SuccNat2Pos.pred_id.
+    erewrite SKINCLGD; cycle 1.
+    { ss. }
+    { apply SKINCL2. }
+    { apply FIND. }
+    { right. left. ss. }
+    hred_r.
+
+    iApply isim_ccallU_mfree.
+    { ss. }
+    { eapply OrdArith.lt_from_nat. lia. }
+    { instantiate (1:=1%ord). eapply OrdArith.lt_from_nat. lia. }
+
+    iPoseProof (list_points_to_collect with "LPT") as (mvs) "[% PT]"; et.
+    rewrite H8 in H15.
+    iPoseProof (points_to_collect with "[PT DATA_PT]") as "PT".
+    { iSplitL "PT". iFrame.
+      rewrite H15.
+      replace (Z.of_nat (esize * length))%nat with (Z.of_nat esize * Z.of_nat length)%Z
+        by (symmetry; apply Nat2Z.inj_mul).
+      iFrame.
+    }
+    iSplitL "INV DATA_HO PT".
+    { iFrame.
+      iExists m_data, (mvs ++ unused). iFrame.
+      iPureIntro. rewrite app_length. lia.
+    }
+
+    iIntros (st_src1 st_tgt1) "INV".
+    hred_r. remove_tau. unhide.
+    change Archi.ptr64 with true. ss.
+    hred_r. remove_tau.
+    rewrite H3. hred_r. rewrite H3. hred_r.
+    replace (alist_find vector._vector ce) with (Some co).
+    hred_r.
+    replace (ClightPlusExprgen.field_offset ce _data (co_members co))
+      with (Errors.OK 0%Z)
+      by (rewrite co_co_members; ss).
+    change (Ptrofs.repr 0) with Ptrofs.zero.
+    rewrite (is_ptr_val_null_r); ss.
+    hred_r.
+
+    rewrite cast_long; ss.
+    change (Vlong (Int64.repr (Int.signed (Int.repr 0)))) with Vnullptr.
+    hred_r.
+
+    iPoseProof (accessor_is_vector_handler_data with "V") as (ofsᵥ) "[DATA V_RECOVER]".
+    rewrite is_ptr_val_null_r; ss.
+    iApply isim_ccallU_store.
+    { ss. }
+    { apply OrdArith.lt_from_nat. lia. }
+    { instantiate (1:=0%ord). apply OrdArith.lt_from_nat. lia. }
+    iSplitL "INV DATA".
+    { iDestruct "DATA" as "[[PT HO] %]". des.
+      iSplitL "INV".
+      - iFrame.
+      - iExists (encode_val Mptr data).
+        iFrame. iPureIntro. ss.
+    }
+    iIntros (st_src2 st_tgt2) "[INV [PT HO]]".
+    hred_r. remove_tau.
+    iPoseProof ("V_RECOVER" with "[PT HO]") as "V". { iFrame; ss. }
+    clear ofsᵥ.
+
+    hred_l.
+    iApply isim_choose_src. iExists (Vundef↑).
+    iApply isim_ret. iFrame. iSplit; ss.
+
+    iDestruct "V" as (ofsᵥ) "(% & PT1 & PT2 & PT3 & PT4 & HO)".
+    rewrite is_ptr_val_null_r; ss.
+    iPoseProof (points_to_collect with "[PT1 PT2]") as "PT". { iSplitL "PT1"; iFrame. }
+    iPoseProof (points_to_collect with "[PT PT3]") as "PT". { iSplitL "PT"; iFrame. }
+    iPoseProof (points_to_collect with "[PT PT4]") as "PT". { iSplitL "PT"; iFrame. }
+    iExists (encode_val Mptr Vnullptr
+               ++ encode_val Mint64 (Vlong (Int64.repr esize))
+               ++ encode_val Mint64 (Vlong (Int64.repr capacity))
+               ++ encode_val Mint64 (Vlong (Int64.repr length))).
+    iExists ofsᵥ. iFrame; ss.
+  Qed.
+
+End PROOF.
