clightplus_examples/vector/vector01proof_vector_esize.v
@@ -1,0 +1,95 @@
+Require Import CoqlibCCR.
+Require Import Any.
+Require Import STS.
+Require Import Behavior.
+Require Import ModSem.
+Require Import SimModSem.
+Require Import PCM.
+Require Import HoareDef.
+Require Import STB.
+Require Import HTactics ProofMode.
+Require Import HSim IProofMode.
+Require Import ClightPlusSkel ClightPlusExprgen ClightPlusgen.
+Require Import ClightPlusMem0 ClightPlusMem1 ClightPlusMemAux.
+Require Import CProofMode CIProofMode.
+Require Import vector.
+Require Import vector0.
+Require Import vector1.
+Require Import PtrofsArith.
+From Coq Require Import Program.
+From compcert Require Import Clightdefs.
+Require Import vector_auxiliary.
+
+Section PROOF.
+
+  Import ClightPlusMem1.
+
+  Context `{@GRA.inG pointstoRA Σ}.
+  Context `{@GRA.inG allocatedRA Σ}.
+  Context `{@GRA.inG blocksizeRA Σ}.
+  Context `{@GRA.inG blockaddressRA Σ}.
+
+  Variable GlobalStb : Sk.t -> gname -> option fspec.
+  Hypothesis STBINCL : forall sk, stb_incl (to_stb vectorStb) (GlobalStb sk).
+  Hypothesis MEMINCL : forall sk, stb_incl (to_stb MemStb) (GlobalStb sk).
+
+  Variable sk: Sk.t.
+  Hypothesis SKINCL1 : Sk.le (vector_compiled.(Mod.sk)) sk.
+  Hypothesis SKINCL2 : Sk.le mfsk sk.
+  Hypothesis SKWF : Sk.wf sk.
+
+  Let ce := Maps.PTree.elements (prog_comp_env prog).
+
+  Lemma sim_vector_esize :
+    sim_fnsem wf top2
+      ("vector_esize", fun_to_tgt "vector" (GlobalStb sk) (mk_pure vector_esize_spec))
+      ("vector_esize", cfunU (decomp_func sk ce f_vector_esize)).
+  Proof.
+    Local Opaque encode_val.
+    Local Opaque cast_to_ptr.
+    econs; ss. red.
+
+    unfold prog, mkprogram in ce.
+    destruct (build_composite_env' composites I). ss.
+    get_composite ce e. fold vector._vector in get_co.
+
+    apply isim_fun_to_tgt; auto. i. simpl in x.
+    destruct x as [[[[[[[[[[[v data] esize] capacity] length] cells] mᵥ] tgᵥ] pᵥ] qᵥ] m_data] q_data].
+    unfold decomp_func, function_entry_c; ss.
+    set (HIDDEN := hide 1).
+
+    iIntros "[INV PRE]".
+    iDestruct "PRE" as "[[% V] %]".
+    clarify. hred_r.
+
+    unhide; change Archi.ptr64 with true; ss. hred_r. remove_tau.
+    iPoseProof (is_vector_fixed_is_ptr_val with "V") as "%".
+    rewrite H3. hred_r. rewrite H3. hred_r.
+    replace (alist_find vector._vector ce) with (Some co) by (apply get_co).
+    hred_r.
+    replace (ClightPlusExprgen.field_offset ce _esize (co_members co)) with (Errors.OK 8%Z)
+      by (rewrite co_co_members; reflexivity).
+    hred_r.
+    iApply isim_apc. iExists (Some (1 : Ord.t)).
+
+    iPoseProof (accessor_is_vector_fixed_is_vector_handler with "V") as ([]) "[VH V_RECOVER]".
+    iPoseProof (accessor_is_vector_handler_esize with "VH") as (ofsᵥ) "[ESIZE VH_RECOVER]".
+    iApply isim_ccallU_load.
+    { ss. }
+    { eapply OrdArith.lt_from_nat. lia. }
+    { instantiate (1:=0%ord). eapply OrdArith.lt_from_nat. lia. }
+    iSplitL "INV ESIZE". { iSplitL "INV"; done. }
+    iIntros (st_src0 st_tgt0) "[INV ESIZE]".
+    iPoseProof ("VH_RECOVER" with "ESIZE") as "VH".
+    iPoseProof ("V_RECOVER" $! () with "VH") as "V".
+
+    Local Transparent cast_to_ptr.
+    hred_r. rewrite decode_encode_item. ss. change Archi.ptr64 with true. ss. hred_r.
+
+    hred_l. iApply isim_choose_src. iExists ((Vlong (Int64.repr esize))↑).
+
+    iApply isim_ret.
+    iSplitL "INV"; et.
+  Qed.
+
+End PROOF.
