clightplus_examples/vector/vector01proof_vector_get.v
@@ -1,0 +1,213 @@
+Require Import CoqlibCCR.
+Require Import Any.
+Require Import STS.
+Require Import Behavior.
+Require Import ModSem.
+Require Import SimModSem.
+Require Import PCM.
+Require Import HoareDef.
+Require Import STB.
+Require Import HTactics ProofMode.
+Require Import HSim IProofMode.
+Require Import ClightPlusSkel ClightPlusExprgen ClightPlusgen.
+Require Import ClightPlusMem0 ClightPlusMem1 ClightPlusMemAux.
+Require Import CProofMode CIProofMode.
+Require Import vector.
+Require Import vector0.
+Require Import vector1.
+Require Import PtrofsArith.
+From Coq Require Import Program.
+From compcert Require Import Clightdefs.
+Require Import vector_auxiliary.
+
+Section PROOF.
+
+  Import ClightPlusMem1.
+
+  Context `{@GRA.inG pointstoRA Σ}.
+  Context `{@GRA.inG allocatedRA Σ}.
+  Context `{@GRA.inG blocksizeRA Σ}.
+  Context `{@GRA.inG blockaddressRA Σ}.
+
+  Variable GlobalStb : Sk.t -> gname -> option fspec.
+  Hypothesis STBINCL : forall sk, stb_incl (to_stb vectorStb) (GlobalStb sk).
+  Hypothesis MEMINCL : forall sk, stb_incl (to_stb MemStb) (GlobalStb sk).
+
+  Variable sk: Sk.t.
+  Hypothesis SKINCL1 : Sk.le (vector_compiled.(Mod.sk)) sk.
+  Hypothesis SKINCL2 : Sk.le mfsk sk.
+  Hypothesis SKWF : Sk.wf sk.
+
+  Let ce := Maps.PTree.elements (prog_comp_env prog).
+
+  Lemma sim_vector_get :
+    sim_fnsem wf top2
+      ("vector_get", fun_to_tgt "vector" (GlobalStb sk) (mk_pure vector_get_spec))
+      ("vector_get", cfunU (decomp_func sk ce f_vector_get)).
+  Proof.
+    Local Opaque encode_val.
+    Local Opaque cast_to_ptr.
+    econs; ss. red.
+
+    unfold prog, mkprogram in ce.
+    destruct (build_composite_env' composites I). ss.
+    get_composite ce e. fold vector._vector in get_co.
+
+    pose proof (incl_incl_env SKINCL1) as SKINCLENV1. unfold incl_env in SKINCLENV1.
+    pose proof (incl_incl_env SKINCL2) as SKINCLENV2. unfold incl_env in SKINCLENV2.
+    pose proof sk_incl_gd as SKINCLGD.
+
+    apply isim_fun_to_tgt; auto. i. simpl in x.
+    destruct x as
+      [[[[[[[[[[[[[[[[[[[
+        [v data] esize] capacity] length] cells] mᵥ] tgᵥ] pᵥ] qᵥ] m_data] q_data]
+        index] mvs_index] p_index] dst] mvs_dst] ofs_dst] m_dst] tg_dst] q_dst].
+    unfold decomp_func, function_entry_c; ss.
+    set (HIDDEN := hide 1).
+
+    iIntros "[INV PRE]".
+    iDestruct "PRE" as "[[% [V [MVS OFS]]] %]". des.
+    revert H6. clarify. i. hred_r.
+
+    unhide. hred_r. remove_tau.
+    unhide. change Archi.ptr64 with true. ss. hred_r. remove_tau.
+    iPoseProof (is_vector_fixed_is_ptr_val with "V") as "%".
+    rewrite H3. hred_r. rewrite H3. hred_r.
+    replace (alist_find vector._vector ce) with (Some co). hred_r.
+    replace (ClightPlusExprgen.field_offset ce _data (co_members co))
+      with (Errors.OK 0%Z)
+      by (rewrite co_co_members; ss).
+    hred_r.
+
+    iPoseProof (is_vector_fixed_is_ptr_data with "V") as "%".
+    iApply isim_apc. iExists (Some (4: Ord.t)).
+    iPoseProof (accessor_is_vector_fixed_is_vector_handler with "V") as ([]) "[VH V_RECOVER]".
+    iPoseProof (accessor_is_vector_handler_data with "VH") as (ofsᵥ) "[DATA VH_RECOVER]".
+    iApply isim_ccallU_load.
+    { ss. }
+    { apply OrdArith.lt_from_nat. lia. }
+    { instantiate (1:=3%ord). apply OrdArith.lt_from_nat. lia. }
+    iSplitL "INV DATA". { iSplitL "INV"; done. }
+    iIntros (st_src0 st_tgt0) "[INV DATA]".
+    iPoseProof ("VH_RECOVER" with "[DATA]") as "VH".
+    { iFrame; ss. }
+    iPoseProof ("V_RECOVER" $! () with "VH") as "V".
+    clear ofsᵥ.
+
+    Local Transparent cast_to_ptr.
+    hred_r.
+    iPoseProof (is_vector_fixed_is_ptr_data with "V") as "%".
+    rewrite (decode_encode_ptr _ H4).
+    rewrite (cast_to_ptr_ptr _ H4).
+    hred_r.
+
+    rewrite H3. hred_r. rewrite H3. hred_r.
+    replace (ClightPlusExprgen.field_offset ce _esize (co_members co))
+      with (Errors.OK 8%Z)
+      by (rewrite co_co_members; ss).
+    hred_r.
+
+    iPoseProof (accessor_is_vector_fixed_is_vector_handler with "V") as ([]) "[VH V_RECOVER]".
+    iPoseProof (accessor_is_vector_handler_esize with "VH") as (ofsᵥ) "[ESIZE VH_RECOVER]".
+    iApply isim_ccallU_load.
+    { ss. }
+    { apply OrdArith.lt_from_nat. lia. }
+    { instantiate (1:=2%ord). apply OrdArith.lt_from_nat. lia. }
+    iDestruct "ESIZE" as "[ESIZE %]".
+    iSplitL "INV ESIZE". { iSplitL "INV". done. iSplit; done. }
+    iIntros (st_src1 st_tgt1) "[INV ESIZE]".
+
+    rewrite decode_encode_item. hred_r.
+    unfold sem_mul_c. ss.
+    change Archi.ptr64 with true. hred_r.
+    rewrite sem_add_ptr_long_c_addl; ss. hred_r.
+    rewrite cast_to_ptr_ptr.
+      2: { destruct data; ss. }
+    hred_r.
+    remove_tau. unhide. hred_r. remove_tau.
+
+    change Archi.ptr64 with true; ss.
+    hexploit SKINCLENV2. { right. right. left. ss. }
+    i. des. rewrite FIND. hred_r.
+    rewrite H3. hred_r. rewrite H3. ss.
+    replace (alist_find vector._vector ce) with (Some co). hred_r.
+    replace (ClightPlusExprgen.field_offset ce _esize (co_members co))
+      with (Errors.OK 8%Z)
+      by (rewrite co_co_members; ss).
+    hred_r.
+
+    iApply isim_ccallU_load.
+    { ss. }
+    { apply OrdArith.lt_from_nat. lia. }
+    { instantiate (1:=1%ord). apply OrdArith.lt_from_nat. lia. }
+    iSplitL "INV ESIZE". { iSplitL "INV". done. iSplit; done. }
+    iIntros (st_src2 st_tgt2) "[INV ESIZE]".
+    iPoseProof ("VH_RECOVER" with "ESIZE") as "VH".
+    iPoseProof ("V_RECOVER" $! () with "VH") as "V".
+
+    rewrite decode_encode_item. hred_r.
+    change Archi.ptr64 with true. ss. hred_r.
+    iPoseProof (points_to_is_ptr with "MVS") as "%".
+    rewrite ! cast_to_ptr_ptr.
+      2: { destruct data; ss. }
+      2: { ss. }
+    hred_r.
+
+    des_if; ss. hred_r.
+    rewrite SuccNat2Pos.pred_id.
+    erewrite SKINCLGD; cycle 1.
+    { ss. }
+    { apply SKINCL2. }
+    { apply FIND. }
+    { right. right. left. reflexivity. }
+    hred_r.
+
+    replace (Vlong (Int64.mul (Int64.repr esize) (Int64.repr index)))
+      with (Vptrofs (Ptrofs.mul (Ptrofs.repr esize) (Ptrofs.repr index))); cycle 1.
+    { unfold Vptrofs. change Archi.ptr64 with true; ss. f_equal.
+      etransitivity.
+      - eapply Ptrofs_to_int64_mul_comm.
+      - f_equal; eapply Ptrofs_to_int64_repr_comm.
+    }
+
+    iApply isim_ccallU_memcpy0.
+    { ss. }
+    { apply OrdArith.lt_from_nat. lia. }
+    { instantiate (1:=0%ord). apply OrdArith.lt_from_nat. lia. }
+
+    iPoseProof (is_vector_fixed_cells_esize with "V") as "%".
+    iPoseProof (is_vector_fixed_esize_range with "V") as "%".
+    iPoseProof (accessor_is_vector_fixed_cells with "V") as ([]) "[[CELLS HO] V_RECOVER]".
+    iPoseProof ((accessor_cells_cell esize data m_data cells index) with "CELLS") as ([]) "[CELL CELLS_RECOVER]"; et.
+    ss.
+
+    iSplitL "MVS OFS INV HO CELL".
+    { iFrame.
+      iExists mvs_dst.
+      iFrame.
+      iSplit.
+      - iPureIntro. splits.
+        + eapply Forall_lookup_1 in H13; et. ss. congruence.
+        + rewrite Int64.unsigned_repr.
+          * rewrite Nat2Z.id. ss.
+          * lia.
+        + left. ss.
+        + apply Z.divide_1_l.
+        + apply Z.divide_1_l.
+        + rewrite Int64.unsigned_repr; lia.
+        + apply Z.divide_1_l.
+      - iApply offset_slide. iFrame.
+    }
+    iIntros (st_src3 st_tgt3) "[INV [[[HO OFS] CELL] MVS]]".
+    iPoseProof (offset_slide_rev with "HO") as "HO".
+    iPoseProof ("CELLS_RECOVER" $! () with "CELL") as "CELLS".
+    iPoseProof ("V_RECOVER" $! () with "[CELLS HO]") as "V". { iFrame. }
+    hred_r. remove_tau.
+
+    hred_l.
+    iApply isim_choose_src. iExists (Vundef↑).
+    iApply isim_ret.
+    iFrame. iPureIntro. ss.
+  Qed.
+
+End PROOF.
