clightplus_examples/vector/vector_auxiliary.v
@@ -1,0 +1,608 @@
+Require Import CoqlibCCR.
+Require Import Any.
+Require Import STS.
+Require Import Behavior.
+Require Import ModSem.
+Require Import SimModSem.
+Require Import PCM.
+Require Import HoareDef.
+Require Import STB.
+Require Import HTactics ProofMode.
+Require Import HSim IProofMode.
+Require Import ClightPlusSkel ClightPlusExprgen ClightPlusgen.
+Require Import ClightPlusMem0 ClightPlusMem1 ClightPlusMemAux.
+Require Import CProofMode CIProofMode.
+Require Import vector1.
+Require Import PtrofsArith.
+From Coq Require Import Program.
+From compcert Require Import Clightdefs.
+
+Section INTEGERS.
+
+  Instance eqmod_Reflexive m : Reflexive (Zbits.eqmod m).
+  Proof. exact (Zbits.eqmod_refl m). Qed.
+
+  Instance eqmod_Symmetric m : Symmetric (Zbits.eqmod m).
+  Proof. exact (Zbits.eqmod_sym m). Qed.
+
+  Instance eqmod_Transitive m : Transitive (Zbits.eqmod m).
+  Proof. exact (Zbits.eqmod_trans m). Qed.
+
+  Lemma divide_iff_eqmod_0 m n : (m | n)%Z <-> Zbits.eqmod m n 0.
+  Proof.
+    unfold Zbits.eqmod. unfold Z.divide. split.
+    - intros [k H]. exists k. lia.
+    - intros [k H]. exists k. lia.
+  Qed.
+
+  Lemma Ptrofs_repr_add_comm x y :
+    Ptrofs.repr (x + y) = Ptrofs.add (Ptrofs.repr x) (Ptrofs.repr y).
+  Proof.
+    unfold Ptrofs.add.
+    eapply Ptrofs.eqm_samerepr.
+    eapply Ptrofs.eqm_add; eapply Ptrofs.eqm_unsigned_repr.
+  Qed.
+
+  Lemma Ptrofs_repr_mul_comm x y :
+    Ptrofs.repr (x * y) = Ptrofs.mul (Ptrofs.repr x) (Ptrofs.repr y).
+  Proof.
+    unfold Ptrofs.mul.
+    eapply Ptrofs.eqm_samerepr.
+    eapply Ptrofs.eqm_mult; eapply Ptrofs.eqm_unsigned_repr.
+  Qed.
+
+  Lemma Ptrofs_to_int64_repr_comm n :
+    Ptrofs.to_int64 (Ptrofs.repr n) = Int64.repr n.
+  Proof.
+    eapply Ptrofs.agree64_to_int_eq.
+    eapply Ptrofs.agree64_repr; ss.
+  Qed.
+
+  Lemma Ptrofs_to_int64_add_comm m n :
+    Ptrofs.to_int64 (Ptrofs.add m n) = Int64.add (Ptrofs.to_int64 m) (Ptrofs.to_int64 n).
+  Proof.
+    eapply Ptrofs.agree64_to_int_eq.
+    eapply Ptrofs.agree64_add; ss; apply Ptrofs.agree64_to_int; ss.
+  Qed.
+
+  Lemma Ptrofs_to_int64_mul_comm m n :
+    Ptrofs.to_int64 (Ptrofs.mul m n) = Int64.mul (Ptrofs.to_int64 m) (Ptrofs.to_int64 n).
+  Proof.
+    eapply Ptrofs.agree64_to_int_eq.
+    eapply Ptrofs.agree64_mul; ss; apply Ptrofs.agree64_to_int; ss.
+  Qed.
+
+  Lemma offset_add_align
+    align ofs x
+    : (align | Ptrofs.modulus)%Z ->
+      (align | Ptrofs.unsigned ofs)%Z ->
+      (align | Ptrofs.unsigned x)%Z ->
+      (align | Ptrofs.unsigned (Ptrofs.add ofs x))%Z.
+  Proof.
+    intros H0 H1 H2.
+    eapply divide_iff_eqmod_0.
+    unfold Ptrofs.add.
+    transitivity (Ptrofs.unsigned ofs + Ptrofs.unsigned x)%Z.
+    - symmetry.
+      eapply (Zbits.eqmod_divides Ptrofs.modulus); et.
+      eapply Ptrofs.eqm_unsigned_repr.
+    - eapply divide_iff_eqmod_0.
+      eapply Z.divide_add_r; et.
+  Qed.
+
+  Lemma align8_divides_modulus : (8 | Ptrofs.modulus)%Z.
+  Proof.
+    change Ptrofs.modulus with (8 * 2305843009213693952)%Z.
+    eapply Z.divide_factor_l.
+  Qed.
+
+  Lemma Int64_ltu_true
+    x y
+    : Int64.ltu x y = true ->
+      (Int64.unsigned x < Int64.unsigned y)%Z.
+  Proof.
+    intro H. eapply Int64.ltu_inv in H. lia.
+  Qed.
+
+  Lemma Int64_ltu_false
+    x y
+    : Int64.ltu x y = false ->
+      (Int64.unsigned y <= Int64.unsigned x)%Z.
+  Proof.
+    intro H.
+    apply f_equal with (f := negb) in H.
+    rewrite Int64.not_ltu in H. ss.
+    eapply orb_true_iff in H. destruct H.
+    - eapply Int64.ltu_inv in H. lia.
+    - pose proof (Int64.eq_spec y x) as E.
+      rewrite H in E. subst. lia.
+  Qed.
+
+End INTEGERS.
+
+Section LEMMA.
+
+  Lemma f_bind_ret_r E R A (s : A -> itree E R)
+    : (fun a => ` x : R <- (s a);; Ret x) = s.
+  Proof. apply func_ext. i. apply bind_ret_r. Qed.
+
+  Lemma decode_encode_ofs i : decode_val Mint64 (encode_val Mint64 (Vptrofs i)) = Vptrofs i.
+  Proof.
+    pose proof (decode_encode_val_general (Vptrofs i) Mint64 Mint64).
+    unfold Vptrofs in *. des_ifs.
+  Qed.
+
+  Lemma decode_encode_item i : decode_val Mint64 (encode_val Mint64 (Vlong i)) = Vlong i.
+  Proof. apply (decode_encode_val_general (Vlong i) Mint64 Mint64). Qed.
+
+  Lemma decode_encode_null : decode_val Mint64 (encode_val Mint64 Vnullptr) = Vnullptr.
+  Proof. rewrite (decode_encode_val_general Vnullptr Mint64 Mint64). et. Qed.
+
+  Lemma null_zero i : Vptrofs i = Vnullptr -> i = Ptrofs.zero.
+  Proof.
+    unfold Vptrofs, Vnullptr. des_ifs. i.
+    apply (f_equal (fun v: val => match v with Vlong i => i | _ => Int64.zero end)) in H.
+    rewrite <- (Ptrofs.of_int64_to_int64 Heq i). rewrite H. et.
+  Qed.
+
+  Lemma decode_encode_ptr p : is_ptr_val p -> decode_val Mptr (encode_val Mptr p) = p.
+  Proof.
+    intro.
+    pose proof (decode_encode_val_general p Mptr Mptr).
+    destruct p; ss.
+  Qed.
+
+  Lemma is_ptr_val_null_r
+    p : is_ptr_val p -> Val.addl p (Vptrofs Ptrofs.zero) = p.
+  Proof.
+    i.
+    change (Vptrofs Ptrofs.zero) with (Vlong Int64.zero).
+    destruct p; ss.
+    - rewrite Int64.add_zero. ss.
+    - des_ifs. change (Ptrofs.of_int64 Int64.zero) with Ptrofs.zero.
+      rewrite Ptrofs.add_zero. ss.
+  Qed.
+
+  Lemma addl_Vptrofs m n : Val.addl (Vptrofs m) (Vptrofs n) = Vptrofs (Ptrofs.add m n).
+  Proof.
+    unfold Vptrofs; des_ifs; ss. f_equal.
+    symmetry. eapply Ptrofs_to_int64_add_comm.
+  Qed.
+
+  Context `{eventE -< eff}.
+
+  Lemma encode_ptr_bytes_not_pure p : is_ptr_val p -> bytes_not_pure (encode_val Mptr p) = false.
+  Proof. destruct p; ss. Qed.
+
+  Lemma cast_to_ptr_ptr p : is_ptr_val p -> cast_to_ptr p = Ret p.
+  Proof. destruct p; ss. Qed.
+
+  Lemma cast_ptrofs i : cast_to_ptr (Vptrofs i) = Ret (Vptrofs i).
+  Proof. des_ifs. Qed.
+
+  Lemma cast_long i : Archi.ptr64 = true -> cast_to_ptr (Vlong i) = Ret (Vlong i).
+  Proof. ss. Qed.
+
+  Lemma sem_add_ptr_long_c_addl ce p n
+    (PTR : is_ptr_val p)
+    : sem_add_ptr_long_c ce tschar p (Vlong n) = Ret (Val.addl p (Vlong n)).
+  Proof.
+    unfold sem_add_ptr_long_c, Val.addl.
+    change Archi.ptr64 with true; ss.
+    destruct p; ss; repeat f_equal.
+    - rewrite Int64.mul_commut. apply Int64.mul_one.
+    - rewrite Ptrofs.mul_commut. apply Ptrofs.mul_one.
+  Qed.
+
+End LEMMA.
+
+Section KNOWLEDGES. (* pure of persistent facts *)
+
+  Import ClightPlusMem1.
+
+  Context `{@GRA.inG pointstoRA Σ}.
+  Context `{@GRA.inG allocatedRA Σ}.
+  Context `{@GRA.inG blocksizeRA Σ}.
+  Context `{@GRA.inG blockaddressRA Σ}.
+
+  Lemma is_vector_fixed_esize_range
+    v data (esize : nat) capacity length cells mᵥ tgᵥ pᵥ qᵥ m_data q_data
+      : bi_entails
+        (is_vector_fixed v data esize capacity length cells mᵥ tgᵥ pᵥ qᵥ m_data q_data)
+        ⌜(0 < Z.of_nat esize <= Int64.max_unsigned)%Z⌝%I.
+  Proof.
+    iIntros "V".
+    iDestruct "V" as "(% & _ & _ & _)". des.
+    iPureIntro. nia.
+  Qed.
+
+  Lemma is_vector_esize_range
+    v esize capacity length cells mᵥ tgᵥ qᵥ
+    : bi_entails
+      (is_vector v esize capacity length cells mᵥ tgᵥ qᵥ)
+      ⌜(0 < Z.of_nat esize <= Int64.max_unsigned)%Z⌝%I.
+  Proof.
+    iIntros "V".
+    iDestruct "V" as (? ? ? ?) "(% & _ & _ & _ & _)". des.
+    iPureIntro. nia.
+  Qed.
+
+  Lemma is_vector_capacity_range
+    v esize capacity length cells mᵥ tgᵥ qᵥ
+      : bi_entails
+        (is_vector v esize capacity length cells mᵥ tgᵥ qᵥ)
+        ⌜(0 < Z.of_nat capacity <= Int64.max_unsigned)%Z⌝%I.
+  Proof.
+    iIntros "V".
+    iDestruct "V" as (? ? ? ?) "(% & _ & _ & _ & _)". des.
+    iPureIntro. nia.
+  Qed.
+
+  Lemma is_vector_fixed_cells_esize
+    v data esize capacity length cells mᵥ tgᵥ pᵥ qᵥ m_data q_data
+    : bi_entails
+      (is_vector_fixed v data esize capacity length cells mᵥ tgᵥ pᵥ qᵥ m_data q_data)
+      ⌜Forall (fun c => cell_size c = esize) cells⌝%I.
+  Proof.
+    iIntros "V".
+    iDestruct "V" as "(% & _ & _ & _)". des.
+    iPureIntro.
+    ss.
+  Qed.
+
+  Lemma is_vector_fixed_is_ptr_val
+    v data esize capacity length cells mᵥ tgᵥ pᵥ qᵥ m_data q_data
+    : bi_entails
+      (is_vector_fixed v data esize capacity length cells mᵥ tgᵥ pᵥ qᵥ m_data q_data)
+      ⌜is_ptr_val v = true⌝%I.
+  Proof.
+    iIntros "V".
+    iDestruct "V" as "[% [V1 [V2 V3]]]".
+    iDestruct "V1" as (ofsᵥ) "[% [V1.1 V1.2]]".
+    iPoseProof (points_to_is_ptr with "V1.1") as "%".
+    iPureIntro. destruct v; ss.
+  Qed.
+
+  Lemma is_vector_fixed_is_ptr_data
+    v data esize capacity length cells mᵥ tgᵥ pᵥ qᵥ m_data q_data
+    : bi_entails
+      (is_vector_fixed v data esize capacity length cells mᵥ tgᵥ pᵥ qᵥ m_data q_data)
+      ⌜is_ptr_val data = true⌝%I.
+  Proof.
+    iIntros "V".
+    iDestruct "V" as "[% [V1 [V2 V3]]]".
+    iApply (offset_is_ptr with "V3").
+  Qed.
+
+  Lemma is_vector_is_ptr_val
+    v esize capacity length cells mᵥ tgᵥ qᵥ
+    : bi_entails
+      (is_vector v esize capacity length cells mᵥ tgᵥ qᵥ)
+      ⌜is_ptr_val v = true⌝%I.
+  Proof.
+    iIntros "V".
+    iDestruct "V" as (data m_data unused_length unused) "[% [V1 [V2 [V3 V4]]]]".
+    iDestruct "V1" as (ofsᵥ) "[% [V1.1 V1.2]]".
+    iPoseProof (points_to_is_ptr with "V1.1") as "%".
+    iPureIntro. destruct v; ss.
+  Qed.
+
+  Lemma is_vector_handler_is_ptr_data
+    v data esize capacity length mᵥ tgᵥ qᵥ
+    : bi_entails
+      (is_vector_handler v data esize capacity length mᵥ tgᵥ 1 qᵥ)
+      ⌜is_ptr_val data = true⌝%I.
+  Proof.
+    iIntros "VH".
+    iDestruct "VH" as (ofsᵥ) "[% _]".
+    iPureIntro. apply H3.
+  Qed.
+
+  Lemma list_points_to_collect esize p m cs
+    (SIZE : Forall (fun c => cell_size c = esize) cs)
+    (OWNED : Forall (fun c => exists mvs, c = owned mvs 1) cs) :
+    bi_entails
+      (list_points_to p m cs)
+      (∃ mvs, ⌜Datatypes.length mvs = (esize * Datatypes.length cs)%nat⌝ ∗ p (↦_m, 1) mvs).
+  Proof.
+    revert p.
+    induction cs; i; iIntros "LPT".
+    - iExists []. iSplit; ss.
+    - inv SIZE. inv OWNED. ss. des. clarify.
+      iDestruct "LPT" as "[CPT LPT_OFS]".
+      hexploit IHcs; ss. i.
+      iPoseProof (H3 with "LPT_OFS") as "IH".
+      iDestruct "IH" as (mvs') "[% PT]".
+      iPoseProof (points_to_collect with "[CPT PT]") as "PT".
+      { iSplitL "CPT"; iFrame. }
+      iExists (mvs ++ mvs'). iFrame. iPureIntro.
+      rewrite app_length. lia.
+  Qed.
+
+End KNOWLEDGES.
+
+Section ACCESSORS.
+
+  Import ClightPlusMem1.
+
+  Context `{@GRA.inG pointstoRA Σ}.
+  Context `{@GRA.inG allocatedRA Σ}.
+  Context `{@GRA.inG blocksizeRA Σ}.
+  Context `{@GRA.inG blockaddressRA Σ}.
+
+  (* Slightly different variation of iris.proofmode.classes.accesor *)
+  Definition accessor {X Y : Type} (P : X -> iProp) (Q R : X -> Y -> iProp) :=
+    (∃ x : X, P x ∗ (∀ y : Y, Q x y -∗ R x y))%I.
+
+  Lemma accessor_is_vector_is_vector_fixed
+    v esize capacity length cells mᵥ tgᵥ qᵥ
+      : bi_entails
+          (is_vector v esize capacity length cells mᵥ tgᵥ qᵥ)
+          (accessor
+             (fun '(data, m_data) => ⌜Forall (fun c => exists mvs, c = owned mvs 1) cells⌝
+                                ∗ is_vector_fixed v data esize capacity length cells mᵥ tgᵥ 1 qᵥ m_data 1)
+             (fun '(data, m_data) '(qᵥ', cells') => ⌜Forall (fun c => exists mvs, c = owned mvs 1) cells'⌝
+                                               ∗ is_vector_fixed v data esize capacity length cells' mᵥ tgᵥ 1 qᵥ' m_data 1)
+             (fun '(data, m_data) '(qᵥ', cells') => is_vector v esize capacity length cells' mᵥ tgᵥ qᵥ'))%I.
+  Proof.
+    iIntros "V".
+    iDestruct "V" as (data m_data unused_length unused) "[% [V1 [V2 [V3 V4]]]]"; des.
+    iExists (data, m_data). iSplitL "V1 V2 V3".
+    - iSplit; ss. iFrame. iPureIntro. splits; ss; lia.
+    - iIntros ([qᵥ' cells']) "[% V]".
+      iDestruct "V" as "[% [V1 [V2 V3]]]"; des.
+      iExists data, m_data, (capacity - length), unused.
+      iFrame. iPureIntro. splits; ss; lia.
+  Qed.
+
+  Lemma accessor_is_vector_fixed_is_vector_handler
+    v data esize capacity length cells mᵥ tgᵥ pᵥ qᵥ m_data q_data
+      : bi_entails
+          (is_vector_fixed v data esize capacity length cells mᵥ tgᵥ pᵥ qᵥ m_data q_data)
+          (accessor
+             (fun '() => is_vector_handler v data esize capacity length mᵥ tgᵥ pᵥ qᵥ)
+             (fun '() '() => is_vector_handler v data esize capacity length mᵥ tgᵥ pᵥ qᵥ)
+             (fun '() '() => is_vector_fixed v data esize capacity length cells mᵥ tgᵥ pᵥ qᵥ m_data q_data)).
+  Proof.
+    iIntros "V". iDestruct "V" as "(% & V1 & V2 & V3)".
+    iExists tt. iSplitL "V1".
+    - iFrame.
+    - iIntros ([]) "V1". iFrame. ss.
+  Qed.
+
+  (* N.B. : You can not use this for store *)
+  Lemma accessor_is_vector_is_vector_handler
+    v esize capacity length cells mᵥ tgᵥ qᵥ
+      : bi_entails
+          (is_vector v esize capacity length cells mᵥ tgᵥ qᵥ)
+          (accessor
+             (fun data => is_vector_handler v data esize capacity length mᵥ tgᵥ 1 qᵥ)
+             (fun data '() => is_vector_handler v data esize capacity length mᵥ tgᵥ 1 qᵥ)
+             (fun data '() => is_vector v esize capacity length cells mᵥ tgᵥ qᵥ))%I.
+  Proof.
+    iIntros "V". iDestruct "V" as (data m_data unused_length unused) "(% & V1 & V2 & V3 & V4)".
+    iExists data. iSplitL "V1".
+    - iFrame.
+    - iIntros ([]) "V1". iExists data, m_data, unused_length, unused. iFrame. ss.
+  Qed.
+
+  Lemma accessor_is_vector_handler_data
+    v data esize capacity length mᵥ tgᵥ pᵥ qᵥ
+    : bi_entails
+        (is_vector_handler v data esize capacity length mᵥ tgᵥ pᵥ qᵥ)
+        (accessor
+           (fun ofsᵥ => ( Val.addl v (Vptrofs (Ptrofs.repr 0)) (↦_mᵥ,pᵥ) (encode_val Mptr data)
+                     ∗ Val.addl v (Vptrofs (Ptrofs.repr 0)) (⊨_mᵥ,tgᵥ,qᵥ) ofsᵥ)
+                   ∗ ⌜ strings.length (encode_val Mptr data) = size_chunk_nat Mptr
+                     ∧ bytes_not_pure (encode_val Mptr data) = false
+                     ∧ Mptr ≠ Many64
+                     ∧ (size_chunk Mptr | Ptrofs.unsigned ofsᵥ)%Z
+                     ⌝)
+           (fun ofsᵥ (data' : val) => ( Val.addl v (Vptrofs (Ptrofs.repr 0)) (↦_mᵥ,pᵥ) (encode_val Mptr data')
+                                   ∗ Val.addl v (Vptrofs (Ptrofs.repr 0)) (⊨_mᵥ,tgᵥ,qᵥ) ofsᵥ)
+                                 ∗ ⌜is_ptr_val data'⌝)
+           (fun ofsᵥ (data' : val) => is_vector_handler v data' esize capacity length mᵥ tgᵥ pᵥ qᵥ))%I.
+  Proof.
+    iIntros "V". iDestruct "V" as (ofsᵥ) "(% & PT1 & PT2 & PT3 & PT4 & HO)"; des.
+    iPoseProof (offset_slide with "HO") as "HO".
+    iExists (Ptrofs.add ofsᵥ (Ptrofs.repr 0)).
+    replace (strings.length (encode_val Mptr data)) with 8
+      by (rewrite encode_val_length; ss).
+    iSplitL "PT1 HO".
+    - iFrame. iPureIntro. splits; ss.
+      + apply encode_ptr_bytes_not_pure; ss.
+      + rewrite Ptrofs.add_zero; ss.
+    - iIntros (data') "[[PT1 HO] %]".
+      iPoseProof (offset_slide_rev with "HO") as "HO".
+      iExists ofsᵥ. iFrame. ss.
+  Qed.
+
+  Lemma accessor_is_vector_handler_esize
+    v data esize capacity length mᵥ tgᵥ pᵥ qᵥ
+    : bi_entails
+        (is_vector_handler v data esize capacity length mᵥ tgᵥ pᵥ qᵥ)
+        (accessor
+           (fun ofsᵥ => ( Val.addl v (Vptrofs (Ptrofs.repr 8)) (↦_mᵥ,pᵥ) encode_val Mint64 (Vlong (Int64.repr esize))
+                     ∗ Val.addl v (Vptrofs (Ptrofs.repr 8)) (⊨_mᵥ,tgᵥ,qᵥ) ofsᵥ)
+                   ∗ ⌜ strings.length (encode_val Mint64 (Vlong (Int64.repr esize))) = size_chunk_nat Mint64
+                     ∧ bytes_not_pure (encode_val Mint64 (Vlong (Int64.repr esize))) = false
+                     ∧ Mint64 ≠ Many64
+                     ∧ (size_chunk Mint64 | Ptrofs.unsigned ofsᵥ)%Z
+                     ⌝)
+           (fun ofsᵥ (esize' : nat) => Val.addl v (Vptrofs (Ptrofs.repr 8)) (↦_mᵥ,pᵥ) encode_val Mint64 (Vlong (Int64.repr esize'))
+                                ∗ Val.addl v (Vptrofs (Ptrofs.repr 8)) (⊨_mᵥ,tgᵥ,qᵥ) ofsᵥ)
+           (fun ofsᵥ (esize' : nat) => is_vector_handler v data esize' capacity length mᵥ tgᵥ pᵥ qᵥ))%I.
+  Proof.
+    iIntros "V". iDestruct "V" as (ofsᵥ) "(% & PT1 & PT2 & PT3 & PT4 & HO)"; des.
+    iPoseProof (offset_slide with "HO") as "HO".
+    iExists (Ptrofs.add ofsᵥ (Ptrofs.repr 8)).
+    replace (strings.length (encode_val Mint64 (Vlong (Int64.repr esize)))) with 8
+      by (rewrite encode_val_length; ss).
+    iSplitL "PT2 HO".
+    - iFrame. iPureIntro. splits; ss.
+      eapply offset_add_align.
+      + eapply align8_divides_modulus.
+      + et.
+      + change (Ptrofs.unsigned (Ptrofs.repr 8)) with (8*1)%Z.
+        eapply Z.divide_factor_l.
+    - iIntros (esize') "[PT2 HO]".
+      iPoseProof (offset_slide_rev with "HO") as "HO".
+      iExists ofsᵥ. iFrame. ss.
+  Qed.
+
+  Lemma accessor_is_vector_handler_capacity
+    v data esize capacity length mᵥ tgᵥ pᵥ qᵥ
+    : bi_entails
+        (is_vector_handler v data esize capacity length mᵥ tgᵥ pᵥ qᵥ)
+        (accessor
+           (fun ofsᵥ => ( Val.addl v (Vptrofs (Ptrofs.repr 16)) (↦_mᵥ,pᵥ) encode_val Mint64 (Vlong (Int64.repr capacity))
+                     ∗ Val.addl v (Vptrofs (Ptrofs.repr 16)) (⊨_mᵥ,tgᵥ,qᵥ) ofsᵥ)
+                   ∗ ⌜ strings.length (encode_val Mint64 (Vlong (Int64.repr capacity))) = size_chunk_nat Mint64
+                     ∧ bytes_not_pure (encode_val Mint64 (Vlong (Int64.repr capacity))) = false
+                     ∧ Mint64 ≠ Many64
+                     ∧ (size_chunk Mint64 | Ptrofs.unsigned ofsᵥ)%Z
+                     ⌝)
+           (fun ofsᵥ (capacity' : nat) => Val.addl v (Vptrofs (Ptrofs.repr 16)) (↦_mᵥ,pᵥ) encode_val Mint64 (Vlong (Int64.repr capacity'))
+                                   ∗ Val.addl v (Vptrofs (Ptrofs.repr 16)) (⊨_mᵥ,tgᵥ,qᵥ) ofsᵥ)
+           (fun ofsᵥ (capacity' : nat) => is_vector_handler v data esize capacity' length mᵥ tgᵥ pᵥ qᵥ))%I.
+  Proof.
+    iIntros "V". iDestruct "V" as (ofsᵥ) "(% & PT1 & PT2 & PT3 & PT4 & HO)"; des.
+    iPoseProof (offset_slide with "HO") as "HO".
+    iExists (Ptrofs.add ofsᵥ (Ptrofs.repr 16)).
+    replace (strings.length (encode_val Mint64 (Vlong (Int64.repr capacity)))) with 8
+      by (rewrite encode_val_length; ss).
+    iSplitL "PT3 HO".
+    - iFrame. iPureIntro. splits; ss.
+      eapply offset_add_align.
+      + eapply align8_divides_modulus.
+      + et.
+      + change (Ptrofs.unsigned (Ptrofs.repr 16)) with (8*2)%Z.
+        eapply Z.divide_factor_l.
+    - iIntros (esize') "[PT3 HO]".
+      iPoseProof (offset_slide_rev with "HO") as "HO".
+      iExists ofsᵥ. iFrame. ss.
+  Qed.
+
+  Lemma accessor_is_vector_handler_length
+    v data esize capacity length mᵥ tgᵥ pᵥ qᵥ
+    : bi_entails
+        (is_vector_handler v data esize capacity length mᵥ tgᵥ pᵥ qᵥ)
+        (accessor
+           (fun ofsᵥ => ( Val.addl v (Vptrofs (Ptrofs.repr 24)) (↦_mᵥ,pᵥ) encode_val Mint64 (Vlong (Int64.repr length))
+                     ∗ Val.addl v (Vptrofs (Ptrofs.repr 24)) (⊨_mᵥ,tgᵥ,qᵥ) ofsᵥ)
+                   ∗ ⌜ strings.length (encode_val Mint64 (Vlong (Int64.repr length))) = size_chunk_nat Mint64
+                     ∧ bytes_not_pure (encode_val Mint64 (Vlong (Int64.repr length))) = false
+                     ∧ Mint64 ≠ Many64
+                     ∧ (size_chunk Mint64 | Ptrofs.unsigned ofsᵥ)%Z
+                     ⌝)
+           (fun ofsᵥ (length' : nat) => Val.addl v (Vptrofs (Ptrofs.repr 24)) (↦_mᵥ,pᵥ) encode_val Mint64 (Vlong (Int64.repr length'))
+                                 ∗ Val.addl v (Vptrofs (Ptrofs.repr 24)) (⊨_mᵥ,tgᵥ,qᵥ) ofsᵥ)
+           (fun ofsᵥ (length' : nat) => is_vector_handler v data esize capacity length' mᵥ tgᵥ pᵥ qᵥ))%I.
+  Proof.
+    iIntros "V". iDestruct "V" as (ofsᵥ) "(% & PT1 & PT2 & PT3 & PT4 & HO)"; des.
+    iPoseProof (offset_slide with "HO") as "HO".
+    iExists (Ptrofs.add ofsᵥ (Ptrofs.repr 24)).
+    replace (strings.length (encode_val Mint64 (Vlong (Int64.repr length)))) with 8
+      by (rewrite encode_val_length; ss).
+    iSplitL "PT4 HO".
+    - iFrame. iPureIntro. splits; ss.
+      eapply offset_add_align.
+      + eapply align8_divides_modulus.
+      + et.
+      + change (Ptrofs.unsigned (Ptrofs.repr 24)) with (8*3)%Z.
+        eapply Z.divide_factor_l.
+    - iIntros (esize') "[PT4 HO]".
+      iPoseProof (offset_slide_rev with "HO") as "HO".
+      iExists ofsᵥ. iFrame. ss.
+  Qed.
+
+  Lemma accessor_is_vector_fixed_cells
+    v data esize capacity length cells mᵥ tgᵥ pᵥ qᵥ m_data q_data
+    : bi_entails
+        (is_vector_fixed v data esize capacity length cells mᵥ tgᵥ pᵥ qᵥ m_data q_data)
+        (accessor
+           (fun '() => list_points_to data m_data cells ∗ data (⊨_m_data,Dynamic,q_data) Ptrofs.zero)
+           (fun '() '() => list_points_to data m_data cells ∗ data (⊨_m_data,Dynamic,q_data) Ptrofs.zero)
+           (fun '() '() => is_vector_fixed v data esize capacity length cells mᵥ tgᵥ pᵥ qᵥ m_data q_data))%I.
+  Proof.
+    iIntros "V". iDestruct "V" as "(% & V1 & V2 & V3)"; des.
+    iExists (). iSplitL "V2 V3".
+    - iFrame.
+    - iIntros ([]) "[V2 V3]". iFrame. ss.
+  Qed.
+
+  Lemma accessor_cells_cell
+    esize p m cells (i : nat) cell
+    : is_ptr_val p ->
+      Forall (fun c => cell_size c = esize) cells ->
+      cells !! i = Some cell ->
+      bi_entails
+        (list_points_to p m cells)
+        (accessor
+           (fun '() => cell_points_to (Val.addl p (Vptrofs (Ptrofs.mul (Ptrofs.repr esize) (Ptrofs.repr i)))) m cell)
+           (fun '() '() => cell_points_to (Val.addl p (Vptrofs (Ptrofs.mul (Ptrofs.repr esize) (Ptrofs.repr i)))) m cell)
+           (fun '() '() => list_points_to p m cells))%I.
+  Proof.
+    revert p cells. induction i; i.
+    - destruct cells; ss. inv H5. inversion H4. subst l x. rewrite H7.
+      iIntros "[CELL CELLS]".
+      replace (Ptrofs.mul (Ptrofs.repr esize) (Ptrofs.repr 0)) with Ptrofs.zero
+        by (rewrite Ptrofs.mul_zero; ss).
+      rewrite is_ptr_val_null_r; ss.
+      iExists (). iSplitL "CELL".
+      + iFrame.
+      + iIntros ([]) "CELL". iFrame.
+    - destruct cells; ss. inversion H4. subst l x. rewrite H8.
+      iIntros "[C CELLS]".
+      change (Z.pos (Pos.of_succ_nat i)) with (S i : Z).
+      iPoseProof (IHi with "CELLS") as ([]) "[CELL CELLS]"; et. { destruct p; ss. }
+      iExists ().
+      replace (Val.addl (Val.addl p (Vptrofs (Ptrofs.repr esize))) (Vptrofs (Ptrofs.mul (Ptrofs.repr esize) (Ptrofs.repr i))))
+        with (Val.addl p (Vptrofs (Ptrofs.mul (Ptrofs.repr esize) (Ptrofs.repr (S i))))).
+      2: {
+        rewrite Nat2Z.inj_succ. rewrite Val.addl_assoc. f_equal.
+        rewrite addl_Vptrofs. f_equal.
+        replace (Ptrofs.repr esize) with (Ptrofs.mul (Ptrofs.repr esize) Ptrofs.one) at 2
+          by eapply Ptrofs.mul_one.
+        transitivity (Ptrofs.mul (Ptrofs.repr esize) (Ptrofs.add Ptrofs.one (Ptrofs.repr i))).
+        - f_equal. rewrite Ptrofs.add_unsigned.
+           unfold Ptrofs.one, Z.succ.
+           rewrite ! Ptrofs_repr_add_comm.
+           rewrite ! Ptrofs.repr_unsigned.
+           apply Ptrofs.add_commut.
+        - apply Ptrofs.mul_add_distr_r.
+      }
+      iSplitL "CELL".
+      + iFrame.
+      + iIntros ([]) "CELL".
+        iPoseProof ("CELLS" $! () with "CELL") as "CELLS".
+        iFrame.
+  Qed.
+
+End ACCESSORS.
+
+Section PARAMETERS.
+
+  Context `{@GRA.inG pointstoRA Σ}.
+  Context `{@GRA.inG allocatedRA Σ}.
+  Context `{@GRA.inG blocksizeRA Σ}.
+  Context `{@GRA.inG blockaddressRA Σ}.
+
+  Variable GlobalStb : Sk.t -> gname -> option fspec.
+  Hypothesis STBINCL : forall sk, stb_incl (to_stb vectorStb) (GlobalStb sk).
+  Hypothesis MEMINCL : forall sk, stb_incl (to_stb MemStb) (GlobalStb sk).
+
+  Definition wf : _ -> Any.t * Any.t -> Prop :=
+    @mk_wf
+      _
+      unit
+      (fun _ st_src st_tgt => ⌜True⌝)%I.
+
+  Definition mfsk : Sk.t := [("malloc", Gfun (F:=Clight.fundef) (V:=type) (Ctypes.External EF_malloc (Tcons tulong Tnil) (tptr tvoid) cc_default));
+                      ("free", Gfun (Ctypes.External EF_free (Tcons (tptr tvoid) Tnil) tvoid cc_default));
+                      ("memcpy", Gfun(Ctypes.External (EF_external "memcpy" (mksignature (AST.Tlong :: AST.Tlong :: AST.Tlong :: nil) AST.Tlong cc_default))
+                                                    (Tcons (tptr tvoid) (Tcons (tptr tvoid) (Tcons tulong Tnil))) (tptr tvoid) cc_default));
+                      ("realloc", Gfun (Ctypes.External (EF_external "realloc" (mksignature (AST.Tlong :: AST.Tlong :: nil) AST.Tlong cc_default))
+                                                    (Tcons (tptr tvoid) (Tcons tulong Tnil)) (tptr tvoid) cc_default))].
+
+End PARAMETERS.
